big step eval is now heterogenous, as suggested by Zoe.
Existing instances were automatically lifted using typeclass resolution, without any changes to the sourcecode.
Fixed some instances for L6. Checked that translateTo works upto L6 -- the last line in theories/allInstances.v

certicoq/theories/common/certiClasses.v
@@ -5,29 +5,45 @@ Require Import Common.AstCommon.
 
 Class WellFormed (Term: Type) := wf : Term  -> Prop. 
 
-Generalizable Variables Src Dst Inter Term.
+Generalizable Variables Src Dst Inter Term Value SrcValue DstValue InterValue.
 
-(** A [Term] can contain an environment embedded in it. *)
-Class BigStepOpSem (Term:Type) := bigStepEval: Term -> Term -> Prop.
+(** A [Term] can contain an environment embedded in it. 
+Use this class when there is a separate type (and translation?) for values *)
+Class BigStepHetero (Term Value:Type) := bigStepEval: Term -> Value -> Prop.
 
+(** Use this class when values are just a subcollection of terms. *)
+Class BigStepOpSem (Term:Type) := bigStepEvalSame:> BigStepHetero Term Term.
+
+(* In either case, one can use ⇓ to refer to the big step eval relation *)
 
 Notation "s ⇓ t" := (bigStepEval s t) (at level 70).
+
+
 
 Require Import Coq.Unicode.Utf8.
 
 
-Instance liftBigStepException `{BigStepOpSem Term} : BigStepOpSem (exception Term):=
-λ (s sv: exception Term),
+Instance liftBigStepException `{BigStepHetero Term Value} 
+  : BigStepHetero (exception Term) (exception Value) :=
+λ (s : exception Term) (sv : exception Value),
 match (s, sv) with
 | (Ret s, Ret sv) => s ⇓ sv
 | (_,_) => False
 end.
 
 
-Class CerticoqTranslation (Src Dst : Type)
+Class CerticoqTranslation (Src Dst : Type) : Type
   := translate : Src -> exception Dst.
 
+Class CerticoqTotalTranslation (Src Dst : Type) : Type
+  := translateT : Src -> Dst.
+
 Arguments translate  Src Dst {CerticoqTranslation} s.
+Arguments translateT  Src Dst {CerticoqTotalTranslation} s.
+
+Instance liftTotal `{CerticoqTotalTranslation Src Dst} : CerticoqTranslation Src Dst :=
+  fun (x:Src) => Ret (translateT Src Dst x). 
+
 
 Definition wfPreserving `{CerticoqTranslation Src Dst}
     `{WellFormed Src} `{WellFormed Dst} : Prop := 
@@ -40,37 +56,9 @@ Definition wfPreserving `{CerticoqTranslation Src Dst}
 
 Arguments wfPreserving Src Dst {H} {H0} {H1}.
 
-Definition bigStepPreserving `{CerticoqTranslation Src Dst}
-   `{BigStepOpSem Src} `{BigStepOpSem Dst} `{WellFormed Src}
-  :=
-   ∀ (s sv:Src), 
-    wf s 
-    -> s ⇓ sv
-    -> (translate Src Dst s) ⇓ (translate Src Dst sv).
-
-Arguments bigStepPreserving Src Dst {H} {H0} {H1} {H2}.
-
-(* Sometimes, the translation of a value may not be a value. 
-For example, in L3 to L4, the environment is translated as let bindings.
-Thus, a value with a non-empty environment will be translated to a term
-whose outermost operator is a let binding and is hence not a value.
-This definition, which is inspired by CPS correct seems weaker, is not strong enough
-to be sensible. For example it is possible that the translation of [s] and [sv] both
-diverge. *)
-Definition bigStepPreservingWeaker `{CerticoqTranslation Src Dst}
-   `{BigStepOpSem Src} `{BigStepOpSem Dst} `{WellFormed Src}
-  :=
-   ∀ (s sv:Src) (tv : Dst), 
-    wf s 
-    -> s ⇓ sv
-    -> ((translate Src Dst s) ⇓ (Ret tv) <-> (translate Src Dst sv) ⇓ (Ret tv)).
-
-Arguments bigStepPreservingWeaker Src Dst {H} {H0} {H1} {H2}.
-
-
 (** A Certicoq language must have an associated bigstep operational semantics and 
   a well formedness predicate (possibly \_.True) *)
-Class CerticoqLanguage (Term : Type) `{BigStepOpSem Term} `{WellFormed Term} := 
+Class CerticoqLanguage `{BigStepHetero Term Value} `{WellFormed Term} := 
 {
   (* Sensible, but not needed yet.
   wfPreserved : forall (s v : Term), 
@@ -81,23 +69,55 @@ Class CerticoqLanguage (Term : Type) `{BigStepOpSem Term} `{WellFormed Term} :=
 }.
 
 (* can be used to get the term type from an instance *)
-Definition cTerm `{CerticoqLanguage Term} : Type := Term.
+Definition cTerm `{CerticoqLanguage Term Value} : Type := Term.
+(* can be used to get the Value type from an instance *)
+Definition cValue `{CerticoqLanguage Term Value} : Type := Term.
 
-Arguments cTerm {Term} {H} {H0} _.
+Arguments cTerm {Term} {Value} {H} {H0} _.
+Arguments cValue {Term} {Value} {H} {H0} _.
 
+Arguments CerticoqLanguage Term {Value} {H} {H0}.
 
+Definition bigStepPreserving `{CerticoqTranslation Src Dst} 
+  `{CerticoqTranslation SrcValue DstValue}
+   `{BigStepHetero Src SrcValue} `{BigStepHetero Dst DstValue} `{WellFormed Src}
+  :=
+   ∀ (s:Src) (sv: SrcValue), 
+    wf s 
+    -> s ⇓ sv
+    -> (translate Src Dst s) ⇓ (translate SrcValue DstValue sv).
 
-Arguments CerticoqLanguage Term {H} {H0}.
+Arguments bigStepPreserving Src Dst {H} {SrcValue} {DstValue} {H0} {H1} {H2} {H3}.
+
+(* Sometimes, the translation of a value may not be a value. 
+For example, in L3 to L4, the environment is translated as let bindings.
+Thus, a value with a non-empty environment will be translated to a term
+whose outermost operator is a let binding and is hence not a value.
+This definition, which is inspired by CPS correct seems weaker, is not strong enough
+to be sensible. For example it is possible that the translation of [s] and [sv] both
+diverge. 
+Definition bigStepPreservingWeaker `{CerticoqTranslation Src Dst}
+   `{BigStepOpSem Src} `{BigStepOpSem Dst} `{WellFormed Src}
+  :=
+   ∀ (s sv:Src) (tv : Dst), 
+    wf s 
+    -> s ⇓ sv
+    -> ((translate Src Dst s) ⇓ (Ret tv) <-> (translate Src Dst sv) ⇓ (Ret tv)).
+
+Arguments bigStepPreservingWeaker Src Dst {H} {H0} {H1} {H2}.
+*)
+
 
 Class CerticoqTranslationCorrect 
-  `{CerticoqLanguage Src} `{CerticoqLanguage Dst}
-  `{CerticoqTranslation Src Dst} := 
+  `{CerticoqLanguage Src SrcValue} `{CerticoqLanguage Dst DstValue}
+  `{CerticoqTranslation Src Dst} `{CerticoqTranslation SrcValue DstValue} := 
 {
   certiWfPres : wfPreserving Src Dst;
-  certiBigStepPres : bigStepPreserving Src Dst; (* consider [bigStepPreservingWeaker] *)
+  certiBigStepPres : bigStepPreserving Src Dst;
 }.
 
-Arguments CerticoqTranslationCorrect Src {H} {H0} {H1} Dst {H2} {H3} {H4} {H5}.
+Arguments CerticoqTranslationCorrect 
+  Src {SrcValue} {H} {H0} {H1} Dst {DstValue} {H2} {H3} {H4} {H5} {H6}.
 
 Global Instance composeTranslation `{CerticoqTranslation Src Inter} 
   `{CerticoqTranslation Inter Dst} :
@@ -126,12 +146,14 @@ Proof.
 Qed.
 
 
-Instance composeCerticoqTranslationCorrect (Src Inter Dst: Type)
-  `{CerticoqLanguage Src}
-  `{CerticoqLanguage Inter}
-  `{CerticoqLanguage Dst}
+Instance composeCerticoqTranslationCorrect
+  `{CerticoqLanguage Src SrcValue}
+  `{CerticoqLanguage Inter InterValue}
+  `{CerticoqLanguage Dst DstValue}
   {t1 : CerticoqTranslation Src Inter}
   {t2 : CerticoqTranslation Inter Dst}
+  {t1v : CerticoqTranslation SrcValue InterValue}
+  {t2v : CerticoqTranslation InterValue DstValue}
   {Ht1: CerticoqTranslationCorrect Src Inter}
   {Ht2: CerticoqTranslationCorrect Inter Dst}
     : CerticoqTranslationCorrect Src Dst.
@@ -142,7 +164,7 @@ Proof.
   apply certiBigStepPres0 in Hev;[| assumption].
   apply certiWfPres0 in Hwf.
   unfold composeTranslation, translate in *.
-  destruct (t1 s), (t1 sv); compute in Hev; try contradiction.
+  destruct (t1 s), (t1v sv); compute in Hev; try contradiction.
   apply certiBigStepPres1 in Hev;[| assumption].
   exact Hev.
 Qed.
@@ -151,6 +173,35 @@ Qed.
 Instance  BigStepOpWEnv (Term:Set) (ev: (environ Term) -> Term -> Term -> Prop) :
   BigStepOpSem (Program Term) :=
 fun p1 p2 => ev (env p1) (main p1) (main p2) /\ (env p1 = env p2).
+
+Definition normalizes `{BigStepHetero Term Value} (s:Term): Prop :=
+∃ (sv : Value) , s ⇓ sv.
+
+
+(* Todo : generalize over Coq.Init.Logic.eq. *)
+Definition deterministicBigStep `{BigStepHetero Term Value} :=
+∀ (s :Term) (v1 v2 : Value), s ⇓ v1 -> s ⇓ v2 -> v1 = v2.
+
+Arguments deterministicBigStep Term {Value} {H}.
+
+Definition totalTranslation `{CerticoqTranslation Src Dst} : Prop :=
+  ∀ (s:Src), 
+match translate Src Dst s with
+| Ret _ => True
+| Exc _ => False
+end.
+
+
+Lemma deterministicBigStepLiftExc `{BigStepHetero Term Value}:
+  deterministicBigStep Term
+  -> deterministicBigStep (exception Term).
+Proof.
+  intros Hd ? ? ? He1 He2.
+  destruct s, v1, v2; compute in He1; compute in He2; try contradiction.
+  f_equal.
+  unfold deterministicBigStep in Hd.
+  eapply Hd; eauto.
+Qed.
 
 
 (* A possible replacement for [CerticoqTranslationCorrect] 
@@ -186,51 +237,23 @@ Proof.
 (* ( * ) in Randy's email dated Tue, May 31, 2016 at 10:35 PM EST 
 *) 
 
-Definition bigStepReflecting `{CerticoqTranslation Src Dst}  
-   `{BigStepOpSem Src} `{BigStepOpSem Dst} (s:Src) : Prop :=
- ∀ (td: exception Dst), 
+Definition bigStepReflecting `{CerticoqTranslation Src Dst}
+  `{CerticoqTranslation SrcValue DstValue}  
+   `{BigStepHetero Src SrcValue} `{BigStepHetero Dst DstValue} (s:Src) : Prop :=
+ ∀ (td: exception DstValue), 
     (translate Src Dst s) ⇓ td
-    -> ∃ (d:Src), s ⇓ d ∧ td = translate Src Dst d.
+    -> ∃ (d:SrcValue), s ⇓ d ∧ td = translate SrcValue DstValue d.
 
 
-Arguments bigStepReflecting Src Dst {H} {H0} {H1} s.
+Arguments bigStepReflecting Src Dst {H} {SrcValue} {DstValue} {H0} {H1} {H2} s.
 
-
-
-Definition normalizes `{BigStepOpSem Term} (s:Term): Prop :=
-∃ sv, s ⇓ sv.
-
-
-(* Todo : generalize over Coq.Init.Logic.eq. *)
-Definition deterministicBigStep `{BigStepOpSem Term} :=
-∀ (s v1 v2:Term), s ⇓ v1 -> s ⇓ v2 -> v1 = v2.
-
-Arguments deterministicBigStep Term {H}.
-
-Definition totalTranslation `{CerticoqTranslation Src Dst} : Prop :=
-  ∀ (s:Src), 
-match translate Src Dst s with
-| Ret _ => True
-| Exc _ => False
-end.
-
-
-Lemma deterministicBigStepLiftExc `{BigStepOpSem Term}:
-  deterministicBigStep Term
-  -> deterministicBigStep (exception Term).
-Proof.
-  intros Hd ? ? ? He1 He2.
-  destruct s, v1, v2; compute in He1; compute in He2; try contradiction.
-  f_equal.
-  unfold deterministicBigStep in Hd.
-  eapply Hd; eauto.
-Qed.
 
 Lemma bigStepPreservingReflecting 
   `{CerticoqTranslation Src Dst}
-  `{CerticoqLanguage Src}
-  `{BigStepOpSem Dst}
-  `{@bigStepPreserving Src Dst _ _ _ _ } :
+  `{CerticoqTranslation SrcValue DstValue}
+  `{CerticoqLanguage Src SrcValue}
+  `{CerticoqLanguage Dst DstValue}
+  {_:bigStepPreserving Src Dst} :
   (deterministicBigStep Dst)
   -> ∀ (s:Src), 
     wf s
